generic/Zeta.Generic.Interleave.fst
@@ -1,0 +1,33 @@
+module Zeta.Generic.Interleave
+
+
+let lemma_prefix_verifiable (#vspec:_) (n:_) (il:verifiable_log vspec n) (i:nat{i <= S.length il}):
+  Lemma (ensures (verifiable (I.prefix il i)))
+  = admit()
+
+let idxn_has_prefix_prop (#vspec:_) (#n:nat) (#b:_) (tfn: T.idxfn_t vspec b)
+  : Lemma (ensures (IF.prefix_property #(gen_seq vspec n) (idxfn_base #_ #n #_ tfn)))
+  = admit()
+
+let idxfn_prefix_property (#vspec:_) (#n:_) (#b:_) (tfn: T.idxfn_t vspec b)
+  (il: verifiable_log vspec n) (j:nat{j <= S.length il}) (i: nat{i < j})
+  : Lemma (ensures (idxfn tfn il i = idxfn tfn (prefix il j) i))
+  = admit()
+
+let cond_idxfn_has_prefix_prop (#vspec #n #b #f:_) (m: T.cond_idxfn_t b f)
+  : Lemma (ensures (IF.cond_prefix_property #(gen_seq vspec n) #_ #(idxfn f) (cond_idxfn_base m)))
+  = admit()
+
+(*
+  let gs = gen_seq vspec n in
+    //let b = timestamp in
+    let f: IF.idxfn_t gs _ = clock #vspec #n in
+    let s: gs.seq_t = il in
+    //assert(IF.prefix_property f);
+    //assert(j <= gs.length s);
+    //assert(i < j);
+    assert(f s i = f (gs.prefix s j) i);
+    //assert(f s i = clock il i);
+    //assert(f (gs.prefix s j) i = clock (prefix il j) i);
+    ()
+    *)
