utils/Zeta.Interleave.fst
@@ -84,12 +84,13 @@ let lemma_length0_implies_empty (#a #n:_) (il: interleaving a n{length il = 0})
 
 let lemma_empty_sseq (a:eqtype) (n:_) (i: nat{i < n})
   : Lemma (ensures (let il = empty_interleaving a n in
-                    S.index (s_seq il) i = empty #a))
+                    S.index (s_seq il) i = S.empty #a))
   = admit()
 
 let interleaving_extend (#a #n:_) (il: interleaving a n) (x: a) (t: nat{t < n})
   : il': interleaving a n {length il' = length il + 1 /\
                            index il' (length il) = x /\
                            src il' (length il) = t /\
-                           prefix il' (length il) = il}
+                           prefix il' (length il) = il /\
+                           s_seq il' = sseq_extend (s_seq il) x t}
   = admit()
